converted legacy ML script;

src/HOL/UNITY/Comp/Alloc.thy
@@ -259,6 +259,853 @@ locale System =
 		  (plam x: lessThan Nclients. rename client_map Client))"
 **)
 
-ML {* use_legacy_bindings (the_context ()) *}
+(*Perhaps equalities.ML shouldn't add this in the first place!*)
+declare image_Collect [simp del]
+
+declare subset_preserves_o [THEN [2] rev_subsetD, intro]
+declare subset_preserves_o [THEN [2] rev_subsetD, simp]
+declare funPair_o_distrib [simp]
+declare Always_INT_distrib [simp]
+declare o_apply [simp del]
+
+(*For rewriting of specifications related by "guarantees"*)
+lemmas [simp] =
+  rename_image_constrains
+  rename_image_stable
+  rename_image_increasing
+  rename_image_invariant
+  rename_image_Constrains
+  rename_image_Stable
+  rename_image_Increasing
+  rename_image_Always
+  rename_image_leadsTo
+  rename_image_LeadsTo
+  rename_preserves
+  rename_image_preserves
+  lift_image_preserves
+  bij_image_INT
+  bij_is_inj [THEN image_Int]
+  bij_image_Collect_eq
+
+ML {*
+(*Splits up conjunctions & intersections: like CONJUNCTS in the HOL system*)
+fun list_of_Int th = 
+    (list_of_Int (th RS conjunct1) @ list_of_Int (th RS conjunct2))
+    handle THM _ => (list_of_Int (th RS IntD1) @ list_of_Int (th RS IntD2))
+    handle THM _ => (list_of_Int (th RS INT_D))
+    handle THM _ => (list_of_Int (th RS bspec))
+    handle THM _ => [th];
+*}
+
+lemmas lessThanBspec = lessThan_iff [THEN iffD2, THEN [2] bspec]
+
+ML {*
+local
+  val lessThanBspec = thm "lessThanBspec"
+in
+fun normalize th = 
+     normalize (th RS spec
+		handle THM _ => th RS lessThanBspec
+		handle THM _ => th RS bspec
+		handle THM _ => th RS (guarantees_INT_right_iff RS iffD1))
+     handle THM _ => th
+end
+*}
+
+(*** bijectivity of sysOfAlloc [MUST BE AUTOMATED] ***)
+ML {*
+val record_auto_tac =
+  auto_tac (claset() addIs [ext] addSWrapper record_split_wrapper, 
+    simpset() addsimps [thm "sysOfAlloc_def", thm "sysOfClient_def",
+      thm "client_map_def", thm "non_dummy_def", thm "funPair_def", thm "o_apply", thm "Let_def"])
+*}
+
+
+lemma inj_sysOfAlloc [iff]: "inj sysOfAlloc"
+  apply (unfold sysOfAlloc_def Let_def)
+  apply (rule inj_onI)
+  apply (tactic record_auto_tac)
+  done
+
+(*We need the inverse; also having it simplifies the proof of surjectivity*)
+lemma inv_sysOfAlloc_eq [simp]: "!!s. inv sysOfAlloc s =  
+             (| allocGiv = allocGiv s,    
+                allocAsk = allocAsk s,    
+                allocRel = allocRel s,    
+                allocState_d.dummy = (client s, dummy s) |)"
+  apply (rule inj_sysOfAlloc [THEN inv_f_eq])
+  apply (tactic record_auto_tac)
+  done
+
+lemma surj_sysOfAlloc [iff]: "surj sysOfAlloc"
+  apply (simp add: surj_iff expand_fun_eq o_apply)
+  apply (tactic record_auto_tac)
+  done
+
+lemma bij_sysOfAlloc [iff]: "bij sysOfAlloc"
+  apply (blast intro: bijI)
+  done
+
+
+(*** bijectivity of sysOfClient ***)
+
+lemma inj_sysOfClient [iff]: "inj sysOfClient"
+  apply (unfold sysOfClient_def)
+  apply (rule inj_onI)
+  apply (tactic record_auto_tac)
+  done
+
+lemma inv_sysOfClient_eq [simp]: "!!s. inv sysOfClient s =  
+             (client s,  
+              (| allocGiv = allocGiv s,  
+                 allocAsk = allocAsk s,  
+                 allocRel = allocRel s,  
+                 allocState_d.dummy = systemState.dummy s|) )"
+  apply (rule inj_sysOfClient [THEN inv_f_eq])
+  apply (tactic record_auto_tac)
+  done
+
+lemma surj_sysOfClient [iff]: "surj sysOfClient"
+  apply (simp add: surj_iff expand_fun_eq o_apply)
+  apply (tactic record_auto_tac)
+  done
+
+lemma bij_sysOfClient [iff]: "bij sysOfClient"
+  apply (blast intro: bijI)
+  done
+
+
+(*** bijectivity of client_map ***)
+
+lemma inj_client_map [iff]: "inj client_map"
+  apply (unfold inj_on_def)
+  apply (tactic record_auto_tac)
+  done
+
+lemma inv_client_map_eq [simp]: "!!s. inv client_map s =  
+             (%(x,y).(|giv = giv x, ask = ask x, rel = rel x,  
+                       clientState_d.dummy = y|)) s"
+  apply (rule inj_client_map [THEN inv_f_eq])
+  apply (tactic record_auto_tac)
+  done
+
+lemma surj_client_map [iff]: "surj client_map"
+  apply (simp add: surj_iff expand_fun_eq o_apply)
+  apply (tactic record_auto_tac)
+  done
+
+lemma bij_client_map [iff]: "bij client_map"
+  apply (blast intro: bijI)
+  done
+
+
+(** o-simprules for client_map **)
+
+lemma fst_o_client_map: "fst o client_map = non_dummy"
+  apply (unfold client_map_def)
+  apply (rule fst_o_funPair)
+  done
+
+ML {* bind_thms ("fst_o_client_map'", make_o_equivs (thm "fst_o_client_map")) *}
+declare fst_o_client_map' [simp]
+
+lemma snd_o_client_map: "snd o client_map = clientState_d.dummy"
+  apply (unfold client_map_def)
+  apply (rule snd_o_funPair)
+  done
+
+ML {* bind_thms ("snd_o_client_map'", make_o_equivs (thm "snd_o_client_map")) *}
+declare snd_o_client_map' [simp]
+
+(** o-simprules for sysOfAlloc [MUST BE AUTOMATED] **)
+
+lemma client_o_sysOfAlloc: "client o sysOfAlloc = fst o allocState_d.dummy "
+  apply (tactic record_auto_tac)
+  done
+
+ML {* bind_thms ("client_o_sysOfAlloc'", make_o_equivs (thm "client_o_sysOfAlloc")) *}
+declare client_o_sysOfAlloc' [simp]
+
+lemma allocGiv_o_sysOfAlloc_eq: "allocGiv o sysOfAlloc = allocGiv"
+  apply (tactic record_auto_tac)
+  done
+
+ML {* bind_thms ("allocGiv_o_sysOfAlloc_eq'", make_o_equivs (thm "allocGiv_o_sysOfAlloc_eq")) *}
+declare allocGiv_o_sysOfAlloc_eq' [simp]
+
+lemma allocAsk_o_sysOfAlloc_eq: "allocAsk o sysOfAlloc = allocAsk"
+  apply (tactic record_auto_tac)
+  done
+
+ML {* bind_thms ("allocAsk_o_sysOfAlloc_eq'", make_o_equivs (thm "allocAsk_o_sysOfAlloc_eq")) *}
+declare allocAsk_o_sysOfAlloc_eq' [simp]
+
+lemma allocRel_o_sysOfAlloc_eq: "allocRel o sysOfAlloc = allocRel"
+  apply (tactic record_auto_tac)
+  done
+
+ML {* bind_thms ("allocRel_o_sysOfAlloc_eq'", make_o_equivs (thm "allocRel_o_sysOfAlloc_eq")) *}
+declare allocRel_o_sysOfAlloc_eq' [simp]
+
+(** o-simprules for sysOfClient [MUST BE AUTOMATED] **)
+
+lemma client_o_sysOfClient: "client o sysOfClient = fst"
+  apply (tactic record_auto_tac)
+  done
+
+ML {* bind_thms ("client_o_sysOfClient'", make_o_equivs (thm "client_o_sysOfClient")) *}
+declare client_o_sysOfClient' [simp]
+
+lemma allocGiv_o_sysOfClient_eq: "allocGiv o sysOfClient = allocGiv o snd "
+  apply (tactic record_auto_tac)
+  done
+
+ML {* bind_thms ("allocGiv_o_sysOfClient_eq'", make_o_equivs (thm "allocGiv_o_sysOfClient_eq")) *}
+declare allocGiv_o_sysOfClient_eq' [simp]
+
+lemma allocAsk_o_sysOfClient_eq: "allocAsk o sysOfClient = allocAsk o snd "
+  apply (tactic record_auto_tac)
+  done
+
+ML {* bind_thms ("allocAsk_o_sysOfClient_eq'", make_o_equivs (thm "allocAsk_o_sysOfClient_eq")) *}
+declare allocAsk_o_sysOfClient_eq' [simp]
+
+lemma allocRel_o_sysOfClient_eq: "allocRel o sysOfClient = allocRel o snd "
+  apply (tactic record_auto_tac)
+  done
+
+ML {* bind_thms ("allocRel_o_sysOfClient_eq'", make_o_equivs (thm "allocRel_o_sysOfClient_eq")) *}
+declare allocRel_o_sysOfClient_eq' [simp]
+
+lemma allocGiv_o_inv_sysOfAlloc_eq: "allocGiv o inv sysOfAlloc = allocGiv"
+  apply (simp add: o_def)
+  done
+
+ML {* bind_thms ("allocGiv_o_inv_sysOfAlloc_eq'", make_o_equivs (thm "allocGiv_o_inv_sysOfAlloc_eq")) *}
+declare allocGiv_o_inv_sysOfAlloc_eq' [simp]
+
+lemma allocAsk_o_inv_sysOfAlloc_eq: "allocAsk o inv sysOfAlloc = allocAsk"
+  apply (simp add: o_def)
+  done
+
+ML {* bind_thms ("allocAsk_o_inv_sysOfAlloc_eq'", make_o_equivs (thm "allocAsk_o_inv_sysOfAlloc_eq")) *}
+declare allocAsk_o_inv_sysOfAlloc_eq' [simp]
+
+lemma allocRel_o_inv_sysOfAlloc_eq: "allocRel o inv sysOfAlloc = allocRel"
+  apply (simp add: o_def)
+  done
+
+ML {* bind_thms ("allocRel_o_inv_sysOfAlloc_eq'", make_o_equivs (thm "allocRel_o_inv_sysOfAlloc_eq")) *}
+declare allocRel_o_inv_sysOfAlloc_eq' [simp]
+
+lemma rel_inv_client_map_drop_map: "(rel o inv client_map o drop_map i o inv sysOfClient) =  
+      rel o sub i o client"
+  apply (simp add: o_def drop_map_def)
+  done
+
+ML {* bind_thms ("rel_inv_client_map_drop_map'", make_o_equivs (thm "rel_inv_client_map_drop_map")) *}
+declare rel_inv_client_map_drop_map [simp]
+
+lemma ask_inv_client_map_drop_map: "(ask o inv client_map o drop_map i o inv sysOfClient) =  
+      ask o sub i o client"
+  apply (simp add: o_def drop_map_def)
+  done
+
+ML {* bind_thms ("ask_inv_client_map_drop_map'", make_o_equivs (thm "ask_inv_client_map_drop_map")) *}
+declare ask_inv_client_map_drop_map [simp]
+
+(**
+Open_locale "System"
+
+val Alloc = thm "Alloc";
+val Client = thm "Client";
+val Network = thm "Network";
+val System_def = thm "System_def";
+
+CANNOT use bind_thm: it puts the theorem into standard form, in effect
+  exporting it from the locale
+**)
+
+declare finite_lessThan [iff]
+
+(*Client : <unfolded specification> *)
+lemmas client_spec_simps =
+  client_spec_def client_increasing_def client_bounded_def
+  client_progress_def client_allowed_acts_def client_preserves_def
+  guarantees_Int_right
+
+ML {*
+val [Client_Increasing_ask, Client_Increasing_rel,
+     Client_Bounded, Client_Progress, Client_AllowedActs, 
+     Client_preserves_giv, Client_preserves_dummy] =
+        thm "Client" |> simplify (simpset() addsimps (thms "client_spec_simps") )
+               |> list_of_Int;
+
+bind_thm ("Client_Increasing_ask", Client_Increasing_ask);
+bind_thm ("Client_Increasing_rel", Client_Increasing_rel);
+bind_thm ("Client_Bounded", Client_Bounded);
+bind_thm ("Client_Progress", Client_Progress);
+bind_thm ("Client_AllowedActs", Client_AllowedActs);
+bind_thm ("Client_preserves_giv", Client_preserves_giv);
+bind_thm ("Client_preserves_dummy", Client_preserves_dummy);
+*}
+
+declare
+  Client_Increasing_ask [iff]
+  Client_Increasing_rel [iff]
+  Client_Bounded [iff]
+  Client_preserves_giv [iff]
+  Client_preserves_dummy [iff]
+
+
+(*Network : <unfolded specification> *)
+lemmas network_spec_simps =
+  network_spec_def network_ask_def network_giv_def
+  network_rel_def network_allowed_acts_def network_preserves_def
+  ball_conj_distrib
+
+ML {*
+val [Network_Ask, Network_Giv, Network_Rel, Network_AllowedActs,
+     Network_preserves_allocGiv, Network_preserves_rel, 
+     Network_preserves_ask]  =  
+        thm "Network" |> simplify (simpset() addsimps (thms "network_spec_simps"))
+                |> list_of_Int;
+
+bind_thm ("Network_Ask", Network_Ask);
+bind_thm ("Network_Giv", Network_Giv);
+bind_thm ("Network_Rel", Network_Rel);
+bind_thm ("Network_AllowedActs", Network_AllowedActs);
+bind_thm ("Network_preserves_allocGiv", Network_preserves_allocGiv);
+bind_thm ("Network_preserves_rel", Network_preserves_rel);
+bind_thm ("Network_preserves_ask", Network_preserves_ask);
+*}
+
+declare Network_preserves_allocGiv [iff]
+
+declare
+  Network_preserves_rel [simp]
+  Network_preserves_ask [simp]
+
+declare
+  Network_preserves_rel [simplified o_def, simp]
+  Network_preserves_ask [simplified o_def, simp]
+
+(*Alloc : <unfolded specification> *)
+lemmas alloc_spec_simps =
+  alloc_spec_def alloc_increasing_def alloc_safety_def
+  alloc_progress_def alloc_allowed_acts_def alloc_preserves_def
+
+ML {*
+val [Alloc_Increasing_0, Alloc_Safety, Alloc_Progress, Alloc_AllowedActs,
+     Alloc_preserves_allocRel, Alloc_preserves_allocAsk, 
+     Alloc_preserves_dummy] = 
+        thm "Alloc" |> simplify (simpset() addsimps (thms "alloc_spec_simps")) 
+              |> list_of_Int;
+
+bind_thm ("Alloc_Increasing_0", Alloc_Increasing_0);
+bind_thm ("Alloc_Safety", Alloc_Safety);
+bind_thm ("Alloc_Progress", Alloc_Progress);
+bind_thm ("Alloc_AllowedActs", Alloc_AllowedActs);
+bind_thm ("Alloc_preserves_allocRel", Alloc_preserves_allocRel);
+bind_thm ("Alloc_preserves_allocAsk", Alloc_preserves_allocAsk);
+bind_thm ("Alloc_preserves_dummy", Alloc_preserves_dummy);
+*}
+
+(*Strip off the INT in the guarantees postcondition*)
+ML
+{*
+bind_thm ("Alloc_Increasing", normalize Alloc_Increasing_0)
+*}
+
+declare
+  Alloc_preserves_allocRel [iff]
+  Alloc_preserves_allocAsk [iff]
+  Alloc_preserves_dummy [iff]
+
+
+(** Components lemmas [MUST BE AUTOMATED] **)
+
+lemma Network_component_System: "Network Join  
+      ((rename sysOfClient  
+        (plam x: (lessThan Nclients). rename client_map Client)) Join  
+       rename sysOfAlloc Alloc)  
+      = System"
+  apply (simp add: System_def Join_ac)
+  done
+
+lemma Client_component_System: "(rename sysOfClient  
+       (plam x: (lessThan Nclients). rename client_map Client)) Join  
+      (Network Join rename sysOfAlloc Alloc)  =  System"
+  apply (simp add: System_def Join_ac)
+  done
+
+lemma Alloc_component_System: "rename sysOfAlloc Alloc Join  
+       ((rename sysOfClient (plam x: (lessThan Nclients). rename client_map Client)) Join  
+        Network)  =  System"
+  apply (simp add: System_def Join_ac)
+  done
+
+declare
+  Client_component_System [iff]
+  Network_component_System [iff]
+  Alloc_component_System [iff]
+
+(** These preservation laws should be generated automatically **)
+
+lemma Client_Allowed [simp]: "Allowed Client = preserves rel Int preserves ask"
+  apply (auto simp add: Allowed_def Client_AllowedActs safety_prop_Acts_iff)
+  done
+
+lemma Network_Allowed [simp]: "Allowed Network =         
+        preserves allocRel Int  
+        (INT i: lessThan Nclients. preserves(giv o sub i o client))"
+  apply (auto simp add: Allowed_def Network_AllowedActs safety_prop_Acts_iff)
+  done
+
+lemma Alloc_Allowed [simp]: "Allowed Alloc = preserves allocGiv"
+  apply (auto simp add: Allowed_def Alloc_AllowedActs safety_prop_Acts_iff)
+  done
+
+(*needed in rename_client_map_tac*)
+lemma OK_lift_rename_Client [simp]: "OK I (%i. lift i (rename client_map Client))"
+  apply (rule OK_lift_I)
+  apply auto
+  apply (drule_tac w1 = rel in subset_preserves_o [THEN [2] rev_subsetD])
+  apply (drule_tac [2] w1 = ask in subset_preserves_o [THEN [2] rev_subsetD])
+  apply (auto simp add: o_def split_def)
+  done
+
+
+(*The proofs of rename_Client_Increasing, rename_Client_Bounded and
+  rename_Client_Progress are similar.  All require copying out the original
+  Client property.  A forward proof can be constructed as follows:
+
+  Client_Increasing_ask RS
+      (bij_client_map RS rename_rename_guarantees_eq RS iffD2)
+  RS (lift_lift_guarantees_eq RS iffD2)
+  RS guarantees_PLam_I
+  RS (bij_sysOfClient RS rename_rename_guarantees_eq RS iffD2)
+  |> simplify (simpset() addsimps [lift_image_eq_rename, o_def, split_def, 
+				   surj_rename RS surj_range])
+
+However, the "preserves" property remains to be discharged, and the unfolding
+of "o" and "sub" complicates subsequent reasoning.
+
+The following tactic works for all three proofs, though it certainly looks
+ad-hoc!
+*)
+ML
+{*
+val rename_client_map_tac =
+  EVERY [
+    simp_tac (simpset() addsimps [thm "rename_guarantees_eq_rename_inv"]) 1,
+    rtac (thm "guarantees_PLam_I") 1,
+    assume_tac 2,
+	 (*preserves: routine reasoning*)
+    asm_simp_tac (simpset() addsimps [thm "lift_preserves_sub"]) 2,
+	 (*the guarantee for  "lift i (rename client_map Client)" *)
+    asm_simp_tac
+	(simpset() addsimps [thm "lift_guarantees_eq_lift_inv",
+			     thm "rename_guarantees_eq_rename_inv",
+			     thm "bij_imp_bij_inv", thm "surj_rename" RS thm "surj_range",
+			     thm "inv_inv_eq"]) 1,
+    asm_simp_tac
+        (simpset() addsimps [thm "o_def", thm "non_dummy_def", thm "guarantees_Int_right"]) 1]
+*}
+
+(*Lifting Client_Increasing to systemState*)
+lemma rename_Client_Increasing: "i : I  
+      ==> rename sysOfClient (plam x: I. rename client_map Client) :  
+            UNIV  guarantees   
+            Increasing (ask o sub i o client) Int  
+            Increasing (rel o sub i o client)"
+  apply (tactic rename_client_map_tac)
+  sorry
+
+lemma preserves_sub_fst_lift_map: "[| F : preserves w; i ~= j |]  
+      ==> F : preserves (sub i o fst o lift_map j o funPair v w)"
+  apply (auto simp add: lift_map_def split_def linorder_neq_iff o_def)
+  apply (drule_tac [!] subset_preserves_o [THEN [2] rev_subsetD])
+  apply (auto simp add: o_def)
+  done
+
+lemma client_preserves_giv_oo_client_map: "[| i < Nclients; j < Nclients |]  
+      ==> Client : preserves (giv o sub i o fst o lift_map j o client_map)"
+  apply (case_tac "i=j")
+  apply (simp add: o_def non_dummy_def)
+  sorry
+(*
+  apply (drule Client_preserves_dummy [THEN preserves_sub_fst_lift_map])
+  apply (drule_tac [!] subset_preserves_o [THEN [2] rev_subsetD])
+  apply (simp add: o_def client_map_def)
+  done
+*)
+
+lemma rename_sysOfClient_ok_Network:
+  "rename sysOfClient (plam x: lessThan Nclients. rename client_map Client) 
+    ok Network"
+  apply (auto simp add: ok_iff_Allowed client_preserves_giv_oo_client_map)
+  done
+
+lemma rename_sysOfClient_ok_Alloc:
+  "rename sysOfClient (plam x: lessThan Nclients. rename client_map Client) 
+    ok rename sysOfAlloc Alloc"
+  apply (simp add: ok_iff_Allowed)
+  done
+
+lemma rename_sysOfAlloc_ok_Network: "rename sysOfAlloc Alloc ok Network"
+  apply (simp add: ok_iff_Allowed)
+  done
+
+declare
+  rename_sysOfClient_ok_Network [iff]
+  rename_sysOfClient_ok_Alloc [iff]
+  rename_sysOfAlloc_ok_Network [iff]
+
+(*The "ok" laws, re-oriented*)
+declare
+  rename_sysOfClient_ok_Network [THEN ok_sym, iff]
+  rename_sysOfClient_ok_Alloc [THEN ok_sym, iff]
+  rename_sysOfAlloc_ok_Network [THEN ok_sym]
+
+lemma System_Increasing: "i < Nclients
+      ==> System : Increasing (ask o sub i o client) Int  
+                   Increasing (rel o sub i o client)"
+  apply (rule component_guaranteesD [OF rename_Client_Increasing Client_component_System])
+  apply auto
+  done
+
+lemmas rename_guarantees_sysOfAlloc_I =
+  bij_sysOfAlloc [THEN rename_rename_guarantees_eq, THEN iffD2, standard]
+
+
+(*Lifting Alloc_Increasing up to the level of systemState*)
+ML {*
+bind_thm ("rename_Alloc_Increasing",
+  thm "Alloc_Increasing" RS thm "rename_guarantees_sysOfAlloc_I"
+     |> simplify (simpset() addsimps [thm "surj_rename" RS thm "surj_range", thm "o_def"]))
+*}
+
+lemma System_Increasing_allocGiv: 
+     "i < Nclients ==> System : Increasing (sub i o allocGiv)"
+  apply (unfold System_def)
+  apply (simp add: o_def)
+  sorry
+(*
+  apply (rule rename_Alloc_Increasing [THEN guarantees_Join_I1, THEN guaranteesD])
+  apply auto
+  done
+*)
+
+ML {*
+bind_thms ("System_Increasing'", list_of_Int (thm "System_Increasing"))
+*}
+
+declare System_Increasing' [intro!]
+
+(** Follows consequences.
+    The "Always (INT ...) formulation expresses the general safety property
+    and allows it to be combined using Always_Int_rule below. **)
+
+lemma System_Follows_rel: 
+  "i < Nclients ==> System : ((sub i o allocRel) Fols (rel o sub i o client))"
+  apply (auto intro!: Network_Rel [THEN component_guaranteesD])
+  sorry
+
+lemma System_Follows_ask: 
+  "i < Nclients ==> System : ((sub i o allocAsk) Fols (ask o sub i o client))"
+  sorry
+(*
+  apply (auto intro!: [Network_Ask [THEN component_guaranteesD]])
+  done
+*)
+
+lemma System_Follows_allocGiv: 
+  "i < Nclients ==> System : (giv o sub i o client) Fols (sub i o allocGiv)"
+  apply (auto intro!: Network_Giv [THEN component_guaranteesD]
+    rename_Alloc_Increasing [THEN component_guaranteesD])
+  apply (simp_all add: o_def non_dummy_def)
+  sorry
+(*
+  apply (auto intro!: rename_Alloc_Increasing [THEN component_guaranteesD])
+  done
+*)
+
+lemma Always_giv_le_allocGiv: "System : Always (INT i: lessThan Nclients.  
+                       {s. (giv o sub i o client) s <= (sub i o allocGiv) s})"
+  apply auto
+  sorry
+(*
+  apply (erule System_Follows_allocGiv [THEN Follows_Bounded])
+  done
+*)
+
+lemma Always_allocAsk_le_ask: "System : Always (INT i: lessThan Nclients.  
+                       {s. (sub i o allocAsk) s <= (ask o sub i o client) s})"
+  apply auto
+  sorry
+(*
+  apply (erule System_Follows_ask [THEN Follows_Bounded])
+  done
+*)
+
+lemma Always_allocRel_le_rel: "System : Always (INT i: lessThan Nclients.  
+                       {s. (sub i o allocRel) s <= (rel o sub i o client) s})"
+  sorry
+(*
+  apply (auto intro!: Follows_Bounded System_Follows_rel)
+  done
+*)
+
+(*** Proof of the safety property (1) ***)
+
+(*safety (1), step 1 is System_Follows_rel*)
+
+(*safety (1), step 2*)
+(* i < Nclients ==> System : Increasing (sub i o allocRel) *)
+lemmas System_Increasing_allocRel = System_Follows_rel [THEN Follows_Increasing1, standard]
+
+(*Lifting Alloc_safety up to the level of systemState.
+  Simplififying with o_def gets rid of the translations but it unfortunately
+  gets rid of the other "o"s too.*)
+ML {*
+ val rename_Alloc_Safety = 
+    thm "Alloc_Safety" RS thm "rename_guarantees_sysOfAlloc_I"
+     |> simplify (simpset() addsimps [o_def])
+*}
+
+(*safety (1), step 3*)
+(*
+lemma System_sum_bounded: 
+    "System : Always {s. (\<Sum>i: lessThan Nclients. (tokens o sub i o allocGiv) s)
+            <= NbT + (\<Sum>i: lessThan Nclients. (tokens o sub i o allocRel) s)}"
+  apply (simp add: o_apply)
+  apply (rule rename_Alloc_Safety [THEN component_guaranteesD])
+  apply (auto simp add: o_simp System_Increasing_allocRel)
+  done
+*)
+
+(** Follows reasoning **)
+
+lemma Always_tokens_giv_le_allocGiv: "System : Always (INT i: lessThan Nclients.  
+                          {s. (tokens o giv o sub i o client) s  
+                           <= (tokens o sub i o allocGiv) s})"
+  apply (rule Always_giv_le_allocGiv [THEN Always_weaken])
+  apply (auto intro: tokens_mono_prefix simp add: o_apply)
+  done
+
+lemma Always_tokens_allocRel_le_rel: "System : Always (INT i: lessThan Nclients.  
+                          {s. (tokens o sub i o allocRel) s  
+                           <= (tokens o rel o sub i o client) s})"
+  apply (rule Always_allocRel_le_rel [THEN Always_weaken])
+  apply (auto intro: tokens_mono_prefix simp add: o_apply)
+  done
+
+(*safety (1), step 4 (final result!) *)
+lemma System_safety: "System : system_safety"
+  apply (unfold system_safety_def)
+  sorry
+(*
+  apply (tactic {* rtac (Always_Int_rule [thm "System_sum_bounded",
+    thm "Always_tokens_giv_le_allocGiv", thm "Always_tokens_allocRel_le_rel"] RS
+    thm "Always_weaken") 1 *})
+  apply auto
+  apply (rule setsum_fun_mono [THEN order_trans])
+  apply (drule_tac [2] order_trans)
+  apply (rule_tac [2] add_le_mono [OF order_refl setsum_fun_mono])
+  prefer 3 apply assumption
+  apply auto
+  done
+*)
+
+(*** Proof of the progress property (2) ***)
+
+(*progress (2), step 1 is System_Follows_ask and System_Follows_rel*)
+
+(*progress (2), step 2; see also System_Increasing_allocRel*)
+(* i < Nclients ==> System : Increasing (sub i o allocAsk) *)
+lemmas System_Increasing_allocAsk =  System_Follows_ask [THEN Follows_Increasing1, standard]
+
+(*progress (2), step 3: lifting "Client_Bounded" to systemState*)
+lemma rename_Client_Bounded: "i : I  
+    ==> rename sysOfClient (plam x: I. rename client_map Client) :  
+          UNIV  guarantees   
+          Always {s. ALL elt : set ((ask o sub i o client) s). elt <= NbT}"
+  apply (tactic rename_client_map_tac)
+  sorry
+
+lemma System_Bounded_ask: "i < Nclients  
+      ==> System : Always  
+                    {s. ALL elt : set ((ask o sub i o client) s). elt <= NbT}"
+  apply (rule component_guaranteesD [OF rename_Client_Bounded Client_component_System])
+  apply auto
+  done
+
+lemma Collect_all_imp_eq: "{x. ALL y. P y --> Q x y} = (INT y: {y. P y}. {x. Q x y})"
+  apply blast
+  done
+
+(*progress (2), step 4*)
+lemma System_Bounded_allocAsk: "System : Always {s. ALL i<Nclients.  
+                          ALL elt : set ((sub i o allocAsk) s). elt <= NbT}"
+  apply (auto simp add: Collect_all_imp_eq)
+  apply (tactic {* rtac (Always_Int_rule [thm "Always_allocAsk_le_ask",
+    thm "System_Bounded_ask"] RS thm "Always_weaken") 1 *})
+  apply (auto dest: set_mono)
+  done
+
+(*progress (2), step 5 is System_Increasing_allocGiv*)
+
+(*progress (2), step 6*)
+(* i < Nclients ==> System : Increasing (giv o sub i o client) *)
+lemmas System_Increasing_giv =  System_Follows_allocGiv [THEN Follows_Increasing1, standard]
+
+
+lemma rename_Client_Progress: "i: I  
+   ==> rename sysOfClient (plam x: I. rename client_map Client)  
+        : Increasing (giv o sub i o client)   
+          guarantees  
+          (INT h. {s. h <= (giv o sub i o client) s &  
+                            h pfixGe (ask o sub i o client) s}   
+                  LeadsTo {s. tokens h <= (tokens o rel o sub i o client) s})"
+  apply (tactic rename_client_map_tac)
+  sorry
+(*
+  apply (simp add: Client_Progress [simplified o_def])
+  done
+*)
+
+
+(*progress (2), step 7*)
+lemma System_Client_Progress: 
+  "System : (INT i : (lessThan Nclients).  
+            INT h. {s. h <= (giv o sub i o client) s &  
+                       h pfixGe (ask o sub i o client) s}   
+                LeadsTo {s. tokens h <= (tokens o rel o sub i o client) s})"
+  apply (rule INT_I)
+(*Couldn't have just used Auto_tac since the "INT h" must be kept*)
+  apply (rule component_guaranteesD [OF rename_Client_Progress Client_component_System])
+  apply (auto simp add: System_Increasing_giv)
+  done
+
+(*Concludes
+ System : {s. k <= (sub i o allocGiv) s} 
+          LeadsTo
+          {s. (sub i o allocAsk) s <= (ask o sub i o client) s} Int
+          {s. k <= (giv o sub i o client) s} *)
+(*
+bind_thm ("lemma",
+    [thm "System_Follows_ask" RS thm "Follows_Bounded",
+     thm "System_Follows_allocGiv" RS thm "Follows_LeadsTo"] MRS thm "Always_LeadsToD");
+*)
+
+(*A more complicated variant of the previous one*)
+(*
+val lemma2 = [lemma, 
+	      System_Follows_ask RS Follows_Increasing1 RS IncreasingD]
+             MRS PSP_Stable;
+*)
+
+lemma lemma3: "i < Nclients  
+      ==> System : {s. h <= (sub i o allocGiv) s &       
+                       h pfixGe (sub i o allocAsk) s}    
+                   LeadsTo   
+                   {s. h <= (giv o sub i o client) s &   
+                       h pfixGe (ask o sub i o client) s}"
+  apply (rule single_LeadsTo_I)
+  sorry
+(*
+  apply (rule_tac k6 = "h" and x2 = " (sub i o allocAsk) s" in lemma2 [THEN LeadsTo_weaken])
+  apply auto
+  apply (blast intro: trans_Ge [THEN trans_genPrefix THEN transD] prefix_imp_pfixGe)
+  done
+*)
+
+
+(*progress (2), step 8: Client i's "release" action is visible system-wide*)
+lemma System_Alloc_Client_Progress: "i < Nclients   
+      ==> System : {s. h <= (sub i o allocGiv) s &  
+                       h pfixGe (sub i o allocAsk) s}   
+                   LeadsTo {s. tokens h <= (tokens o sub i o allocRel) s}"
+  apply (rule LeadsTo_Trans)
+   prefer 2
+   apply (drule System_Follows_rel [THEN
+     mono_tokens [THEN mono_Follows_o, THEN [2] rev_subsetD],
+     THEN Follows_LeadsTo])
+   apply (simp add: o_assoc)
+  apply (rule LeadsTo_Trans)
+   apply (cut_tac [2] System_Client_Progress)
+   prefer 2
+   apply (blast intro: LeadsTo_Basis)
+  apply (erule lemma3)
+  done
+
+(*Lifting Alloc_Progress up to the level of systemState*)
+ML {*
+bind_thm ("rename_Alloc_Progress",
+  thm "Alloc_Progress" RS thm "rename_guarantees_sysOfAlloc_I"
+  |> simplify (simpset() addsimps [thm "o_def"]))
+*}
+
+(*progress (2), step 9*)
+lemma System_Alloc_Progress: 
+ "System : (INT i : (lessThan Nclients).  
+            INT h. {s. h <= (sub i o allocAsk) s}   
+                   LeadsTo {s. h pfixLe (sub i o allocGiv) s})"
+  apply (simp only: o_apply sub_def)
+  sorry
+(*
+  apply (rule rename_Alloc_Progress [THEN component_guaranteesD])
+  apply (auto simp add: 
+    System_Increasing_allocRel [simplified o_def]
+    System_Increasing_allocAsk [simplified o_def]
+    System_Bounded_allocAsk [simplified o_def]
+    System_Alloc_Client_Progress [simplified o_def])
+  done
+*)
+
+
+(*progress (2), step 10 (final result!) *)
+lemma System_Progress: "System : system_progress"
+  apply (unfold system_progress_def)
+  apply (cut_tac System_Alloc_Progress)
+  apply (blast intro: LeadsTo_Trans
+    System_Follows_allocGiv [THEN Follows_LeadsTo_pfixLe]
+    System_Follows_ask [THEN Follows_LeadsTo])
+  done
+
+
+(*Ultimate goal*)
+lemma System_correct: "System : system_spec"
+  apply (unfold system_spec_def)
+  apply (blast intro: System_safety System_Progress)
+  done
+
+
+(** SOME lemmas no longer used **)
+
+lemma non_dummy_eq_o_funPair: "non_dummy = (% (g,a,r). (| giv = g, ask = a, rel = r |)) o  
+                              (funPair giv (funPair ask rel))"
+  apply (rule ext)
+  apply (auto simp add: o_def non_dummy_def)
+  done
+
+lemma preserves_non_dummy_eq: "(preserves non_dummy) =  
+      (preserves rel Int preserves ask Int preserves giv)"
+  apply (simp add: non_dummy_eq_o_funPair)
+  apply auto
+    apply (drule_tac w1 = rel in subset_preserves_o [THEN [2] rev_subsetD])
+    apply (drule_tac [2] w1 = ask in subset_preserves_o [THEN [2] rev_subsetD])
+    apply (drule_tac [3] w1 = giv in subset_preserves_o [THEN [2] rev_subsetD])
+    apply (auto simp add: o_def)
+  done
+
+(*Could go to Extend.ML*)
+lemma bij_fst_inv_inv_eq: "bij f ==> fst (inv (%(x, u). inv f x) z) = f z"
+  apply (rule fst_inv_equalityI)
+   apply (rule_tac f = "%z. (f z, ?h z) " in surjI)
+   apply (simp add: bij_is_inj inv_f_f)
+  apply (simp add: bij_is_surj surj_f_inv_f)
+  done
 
 end
